For each language L1 - L3 I have put everything needed to compile a program (omitting correctness proofs) in a file called compile.v
L1_MalechaQuoted/compile.v
L1_5_box/compile.v
L2_typeStripped/compile.v
L3_flattenedApp/compile.v

(Actually, L2 still requires two other files: term.v and program.v,
but I will fix that.)

I updated _CoqProject, and went to compile the entire project.  L1 -
L3 compiled, but

------------------
File "./L4_deBruijn/L3_to_L4.v", line 162, characters 13-39:
Error: The reference malecha_L1.program_Program was not found in the current
------------------

In the best of all worlds, L4 should only look at L3, (and now, I'm
hoping, only at L3.compile.v).

I did change a lot of things around, and program_Program is now in
L1.compile.v instead of in malecha_L1.v. 

L3.unaryApplications.v has long had a program_Program that went from
L0 (Malecha's quoted Coq) to L3.  That old version, also used some
things from L2.  I hope I've now fixed that.

So, again, I'd like to see L3_to_L4.v use only L3.compile.v

Matthieu, let me know if there is a problem with this.

theories/L1_5_box/program.v
@@ -1,71 +1,39 @@
-(***)
+(****)
 Add LoadPath "../common" as Common.
-Add LoadPath "../L2_typeStrippedL1" as L2.
-(***)
+Add LoadPath "../L1_5_box" as L1_5.
+(****)
 
 Require Import Coq.Lists.List.
 Require Import Coq.Strings.String.
 Require Import Coq.Strings.Ascii.
 Require Import Coq.Arith.Compare_dec.
 Require Import Coq.omega.Omega.
-Require Import L2.term.
+Require Import Common.Common.
+Require Import L1_5.compile.
+Require Import L1_5.term.
 
 Local Open Scope string_scope.
 Local Open Scope bool.
 Local Open Scope list.
 Set Implicit Arguments.
 
-(** Inductive types representation **)
-(* a constructor; the string only for human readability *)
-Record Cnstr := mkCnstr { CnstrNm:string; CnstrArity:nat }.
-Definition defaultCnstr := {| CnstrNm:=""; CnstrArity:= 0 |}.
-(* a type is a list of Cnstrs; string only for human readability *)
-Record ityp := mkItyp { itypNm:string; itypCnstrs:list Cnstr }.
-Definition defaultItyp := {| itypNm:=""; itypCnstrs:=nil |}.
-(* a mutual type package is a list of ityps *)
-Definition itypPack := list ityp.
+Definition envClass := AstCommon.envClass Term.
+Definition ecTrm := ecTrm Term.
+Definition ecTyp := ecTyp Term.
+Definition ecAx := ecAx Term.
 
-(** this function for use in translation from L2 to L3 **)
-Fixpoint arity_from_dtyp
-        (npars:nat) (itps:itypPack) (tndx:nat) (cndx:nat) : exception nat :=
-  do ity <- exnNth itps tndx;
-  do itp <- exnNth (itypCnstrs ity) cndx;
-  ret (npars + (CnstrArity itp)).
 
-(** environments and programs: Gregory's type [program] is inside out
-*** so we reverse it and make it an ordinary association list
-**)
-Inductive envClass := 
-| ecTrm (_:Term)
-| ecTyp (_:nat) (_:itypPack)
-| ecAx.
-
-Lemma isAx_dec:
-  forall (e:envClass), e = ecAx \/ e <> ecAx.
-Proof.
-  destruct e.
-  - right. intros h. discriminate.
-  - right. intros h. discriminate.
-  - left. reflexivity.
-Qed.
-      
-
-(** An environ is a list of definitions.
-***  Currently ignoring Axioms
-**)
-Definition environ := list (string * envClass).
-Record Program : Type := mkPgm { main:Term; env:environ }.
-
-Inductive WFaEc: envClass -> Prop :=
+(** all items in an env are application-well-formed **)
+Inductive WFaEc: envClass-> Prop :=
 | wfaecTrm: forall t, WFapp t -> WFaEc (ecTrm t)
 | wfaecTyp: forall n i, WFaEc (ecTyp n i)
-| wfaecAx: WFaEc ecAx.
+| wfaecAx: WFaEc (ecAx).
 
 Inductive WFaEnv: environ -> Prop :=
 | wfaenil: WFaEnv nil
 | wfaecons: forall ec, WFaEc ec -> forall p, WFaEnv p -> 
                    forall nm, WFaEnv ((nm, ec) :: p).
-Hint Constructors WFaEc WFaEnv.
+
 
 Inductive fresh (nm:string) : environ -> Prop :=
 | fcons: forall s p ec,
@@ -105,9 +73,7 @@ Qed.
 
 (*** Common functions for evaluation ***)
 
-(** Lookup an entry in the environment
-*** axioms are currently not allowed
-**)
+(** Lookup an entry in the environment **)
 Inductive Lookup: string -> environ -> envClass -> Prop :=
 | LHit: forall s p t, Lookup s ((s,t)::p) t
 | LMiss: forall s1 s2 p t ec,
@@ -115,29 +81,54 @@ Inductive Lookup: string -> environ -> envClass -> Prop :=
 Hint Constructors Lookup.
 
 Definition LookupDfn s p t := Lookup s p (ecTrm t).
-Definition LookupTyp s p n i := Lookup s p (ecTyp n i).
-Definition LookupAx s p := Lookup s p ecAx.
+Definition LookupTyp s p n i := Lookup s p (ecTyp  n i).
+Definition LookupAx s p := Lookup s p (ecAx).
+
+Lemma Lookup_fresh_neq:
+  forall nm2 p t, Lookup nm2 p t -> forall nm1, fresh nm1 p -> nm1 <> nm2.
+induction 1; intros.
+- inversion H. assumption.
+- apply IHLookup. apply (fresh_tl H1).
+Qed.
+
+Lemma Lookup_weaken:
+  forall s p t, Lookup s p t -> 
+      forall nm ec, fresh nm p -> Lookup s ((nm, ec) :: p) t.
+intros s p t h1 nm ec h2.
+assert (j1:= Lookup_fresh_neq h1 h2). apply LMiss. apply neq_sym. assumption.
+assumption.
+Qed.
+
+Lemma Lookup_dec:
+  forall s p, (exists t, Lookup s p t) \/ (forall t, ~ Lookup s p t).
+Proof.
+  induction p; intros.
+  - right. intros t h. inversion h.
+  - destruct IHp; destruct a; destruct (string_dec s s0); subst.
+    + left. destruct H. exists e. apply LHit.
+    + left. destruct H. exists x. apply LMiss; assumption.
+    + destruct e.
+      * left. exists (ecTrm t). apply LHit.
+      * left. exists (ecTyp n i). apply LHit. 
+      * left. exists ecAx. apply LHit.
+    + right. intros t h. inversion_Clear h. 
+      * elim n. reflexivity.
+      * elim (H t). assumption.
+Qed.
+
 
 (** equivalent functions **)
 Function lookup (nm:string) (p:environ) : option envClass :=
   match p with
    | nil => None
    | cons (s,ec) p => if (string_eq_bool nm s) then Some ec
-                                 else lookup nm p
+                      else lookup nm p
   end.
 
 Function lookupDfn (nm:string) (p:environ) : option Term :=
   match lookup nm p with
-   | Some (ecTrm t) => Some t
+   | Some (AstCommon.ecTrm _ t) => Some t
    | _ => None
-  end.
-
-Function cnstrArity (itpnm:string) (pndx:nat) (cndx:nat) (p:environ)
-                      : exception nat :=
-  match lookup itpnm p with
-    | Some (ecTyp npars itps) => arity_from_dtyp npars itps pndx cndx
-    | Some _ => raise ("L2.cnstrArity; not a type package: " ++ itpnm)
-    | none => raise ("L2.cnstrArity; datatype package not found: " ++ itpnm)
   end.
 
 Lemma Lookup_lookup:
@@ -170,7 +161,7 @@ Lemma LookupDfn_lookupDfn:
                  forall te, t = (ecTrm te) -> lookupDfn nm p = Some te.
 induction 1; intros; subst.
 - unfold lookupDfn, lookup. rewrite (string_eq_bool_rfl s). reflexivity.
-- unfold lookupDfn, lookup. rewrite (string_eq_bool_neq H). 
+- unfold lookupDfn, lookup. rewrite (string_eq_bool_neq H).
   destruct t; apply IHLookup; reflexivity.
 Qed.
 
@@ -181,70 +172,14 @@ functional induction (lookupDfn nm p); intros h; try discriminate.
 - injection h. intros. subst. apply lookup_Lookup. assumption.
 Qed.
 
-Lemma Lookup_single_valued:
+Lemma Lookup_functional:
   forall (nm:string) (p:environ) (t r:envClass),
     Lookup nm p t -> Lookup nm p r -> t = r.
 intros nm p t r h1 h2. 
-assert (j1:= Lookup_lookup h1 (t:=t)).
-assert (j2:= Lookup_lookup h2 (t:=r)).
-rewrite j1 in j2. injection j2; intros; subst; reflexivity. 
+assert (j1:= Lookup_lookup h1).
+assert (j2:= Lookup_lookup h2).
+rewrite j1 in j2. injection j2; intros; subst. reflexivity.
 Qed.
-
-Lemma LookupDfn_single_valued:
-  forall (nm:string) (p:environ) (t r:Term),
-    LookupDfn nm p t -> LookupDfn nm p r -> t = r.
-Proof.
-  unfold LookupDfn. intros nm p t r h1 h2.
-  injection (Lookup_single_valued h1 h2). intuition.
-Qed.
-
-Lemma LookupAx_lookup:
-  forall nm p, Lookup nm p ecAx -> lookup nm p = Some ecAx.
-Proof.
-  intros nm p h. inversion h; subst; simpl.
-  - rewrite (string_eq_bool_rfl nm). reflexivity.
-  - rewrite (string_eq_bool_neq H). rewrite (Lookup_lookup H0).
-    reflexivity.
-Qed.
-
-(***
-Lemma not_lookupDfn_not_LookupDfn:
- forall (nm:string) (p:environ) (t:Term),
-   ~(lookupDfn nm p = Some t) <-> ~(LookupDfn nm p t).
-split; eapply deMorgan_impl.
-- apply (proj2 (lookupDfn_LookupDfn _ _ _ )).
-- apply (proj1 (lookupDfn_LookupDfn _ _ _ )).
-Qed.
-
-Lemma lookupDfn_None_not_LookupDfn:
-  forall (nm:string) (p:environ) (t:Term),
-    lookupDfn nm p = None -> ~(LookupDfn nm p t).
-intros nm p te h. apply (proj1 (not_lookupDfn_not_LookupDfn _ _ _)). 
-intuition. rewrite h in H. discriminate.
-Qed.
-
-Lemma lookupDfn_neq:
-  forall n1 n2 p t, n1 <> n2 ->
-     lookupDfn n1 ((n2, ecConstr t) :: p) = lookupDfn n1 p.
-intros n1 n2 p t h.
-unfold lookupDfn. rewrite (string_eq_bool_neq h). reflexivity.
-Qed.
-
-Lemma LookupDfn_neq:
-  forall n1 n2 p t u, n1 <> n2 ->
-     LookupDfn n1 ((n2, ecConstr t) :: p) u -> LookupDfn n1 p u.
-intros n1 n2 p t u h1 h2.
-apply (proj1 (lookupDfn_LookupDfn _ _ _)).
-erewrite <- (lookupDfn_neq _ _ h1).
-apply (proj2 (lookupDfn_LookupDfn _ _ _)). eassumption.
-Qed.
-
-Lemma lookupDfn_eq:
-  forall n t p, lookupDfn n ((n, ecConstr t) :: p) = Some t.
-intros n t p.
-unfold lookupDfn. rewrite string_eq_bool_rfl. reflexivity.
-Qed.
-***)
 
 
 Lemma Lookup_pres_WFapp:
@@ -266,38 +201,6 @@ Lemma Lookup_strengthen:
 intros nm1 pp t h nm2 ecx px j1 j2. subst. assert (k:= Lookup_lookup h).
 simpl in k. rewrite (string_eq_bool_neq j2) in k.
 apply lookup_Lookup. assumption.
-Qed.
-
-Lemma Lookup_fresh_neq:
-  forall nm2 p t, Lookup nm2 p t -> forall nm1, fresh nm1 p -> nm1 <> nm2.
-induction 1; intros.
-- inversion H. assumption.
-- apply IHLookup. apply (fresh_tl H1).
-Qed.
-
-Lemma Lookup_weaken:
-  forall s p t, Lookup s p t -> 
-      forall nm ec, fresh nm p -> Lookup s ((nm, ec) :: p) t.
-intros s p t h1 nm ec h2.
-assert (j1:= Lookup_fresh_neq h1 h2). apply LMiss. apply neq_sym. assumption.
-assumption.
-Qed.
-
-Lemma Lookup_dec:
-  forall s p, (exists t, Lookup s p t) \/ (forall t, ~ Lookup s p t).
-Proof.
-  induction p; intros.
-  - right. intros t h. inversion h.
-  - destruct IHp; destruct a; destruct (string_dec s s0); subst.
-    + left. destruct H. exists e. apply LHit.
-    + left. destruct H. exists x. apply LMiss; assumption.
-    + destruct e.
-      * left. exists (ecTrm t). apply LHit.
-      * left. exists (ecTyp n i). apply LHit.
-      * left. exists ecAx. apply LHit.
-    + right. intros t h. inversion_Clear h. 
-      * elim n. reflexivity.
-      * elim (H t). assumption.
 Qed.
 
 Lemma fresh_lookup_None: forall nm p, fresh nm p <-> lookup nm p = None.
@@ -365,16 +268,17 @@ Inductive Crct: environ -> nat -> Term -> Prop :=
 | CrctWkTrmTyp: forall n p t s nm, Crct p n t -> CrctTyp p n s ->
            fresh nm p -> forall m, Crct ((nm,ecTyp m s)::p) n t
 | CrctRel: forall n m p, m < n -> Crct p n prop -> Crct p n (TRel m)
-| CrctCast: forall n p t, Crct p n t -> Crct p n (TCast t)
-| CrctProd: forall n p nm bod,
-            Crct p n prop -> Crct p (S n) bod -> Crct p n (TProd nm bod)
-| CrctLam: forall n p nm bod,
-            Crct p n prop -> Crct p (S n) bod -> Crct p n (TLambda nm bod)
-| CrctLetIn: forall n p nm dfn bod,
-         Crct p n dfn -> Crct p (S n) bod -> 
-         Crct p n (TLetIn nm dfn bod)
+| CrctCast: forall n p t ck ty, Crct p n t -> Crct p n ty ->
+                                Crct p n (TCast t ck ty)
+| CrctProd: forall n p nm ty bod,
+              Crct p (S n) bod -> Crct p n ty -> Crct p n (TProd nm ty bod)
+| CrctLam: forall n p nm ty bod,
+             Crct p (S n) bod -> Crct p n ty -> Crct p n (TLambda nm ty bod)
+| CrctLetIn: forall n p nm dfn ty bod,
+         Crct p n dfn -> Crct p (S n) bod -> Crct p n ty -> 
+         Crct p n (TLetIn nm dfn ty bod)
 | CrctApp: forall n p fn a args,
-             ~ (isApp fn) -> Crct p n fn -> Crct p n a -> Crcts p n args -> 
+             ~ (isApp fn) -> Crct p n fn -> Crct p n a -> Crcts p n args ->
              Crct p n (TApp fn a args)
 | CrctConst: forall n p pd nm,
                Crct p n prop -> LookupDfn nm p pd -> Crct p n (TConst nm)
@@ -382,9 +286,9 @@ Inductive Crct: environ -> nat -> Term -> Prop :=
                    Crct p n prop -> LookupTyp ipkgNm p npars itypk ->
                    CrctCnstr itypk inum cnum ->
                    Crct p n (TConstruct (mkInd ipkgNm inum) cnum)
-| CrctCase: forall n p m mch brs,
-              Crct p n mch -> Crcts p n brs ->
-              Crct p n (TCase m mch brs)
+| CrctCase: forall n p m ty mch brs,
+              Crct p n mch -> Crcts p n brs -> Crct p n ty -> 
+              Crct p n (TCase m ty mch brs)
 | CrctFix: forall n p ds m,
              Crct p n prop ->    (** convenient for IH *)
              CrctDs p (n + dlength ds) ds -> Crct p n (TFix ds m)
@@ -395,8 +299,9 @@ with Crcts: environ -> nat -> Terms -> Prop :=
                Crct p n t -> Crcts p n ts -> Crcts p n (tcons t ts)
 with CrctDs: environ -> nat -> Defs -> Prop :=
 | CrctDsNil: forall n p, Crct p n prop -> CrctDs p n dnil
-| CrctDsCons: forall n p dn db dra ds,
-          Crct p n db -> CrctDs p n ds -> CrctDs p n (dcons dn db dra ds)
+| CrctDsCons: forall n p dn dty db dra ds,
+          Crct p n dty -> Crct p n db -> CrctDs p n ds ->
+          CrctDs p n (dcons dn dty db dra ds)
 with CrctTyp: environ -> nat -> itypPack -> Prop := 
 | CrctTypStart: forall n itp, CrctTyp nil n itp
 | CrctTypWk1: forall n p t s nm, CrctTyp p n t -> Crct p n s ->
@@ -408,9 +313,10 @@ Scheme Crct_ind' := Minimality for Crct Sort Prop
   with Crcts_ind' := Minimality for Crcts Sort Prop
   with CrctDs_ind' := Minimality for CrctDs Sort Prop
   with CrctTyp_ind' := Minimality for CrctTyp Sort Prop.
+Combined Scheme CrctCrctsCrctDs_ind from
+         Crct_ind', Crcts_ind', CrctDs_ind'.
 Combined Scheme CrctCrctsCrctDsTyp_ind from
          Crct_ind', Crcts_ind', CrctDs_ind', CrctTyp_ind'.
-Combined Scheme CrctCrctsCrctDs_ind from Crct_ind', Crcts_ind', CrctDs_ind'.
 
 
 Lemma Crct_WFTrm:
@@ -439,10 +345,8 @@ Lemma Crct_up:
   (forall (p:environ) (n:nat) (itp:itypPack), CrctTyp p n itp ->
                                               CrctTyp p (S n) itp).
 Proof.
-  apply CrctCrctsCrctDsTyp_ind; intros; try (solve [constructor; assumption]).
-  - apply CrctRel; try assumption. omega.
-  - eapply CrctConst; eassumption.
-  - eapply CrctConstruct; eassumption.
+  apply CrctCrctsCrctDsTyp_ind; intros;
+  try (econstructor; try omega; eassumption).
 Qed.
 
 Lemma Crct_Sort:
@@ -457,12 +361,13 @@ Qed.
 
 Lemma Crcts_tnil:
   forall p n t, Crct p n t -> Crcts p n tnil.
-induction 1; apply CrctsNil; try assumption;
-try (solve [eapply Crct_Sort; eassumption]).
-- constructor.
-- constructor.
-- apply CrctWkTrmTrm; try assumption. eapply Crct_Sort; eassumption.
-- apply CrctWkTrmTyp; try assumption. eapply Crct_Sort; eassumption.
+Proof.
+  induction 1; apply CrctsNil; try assumption;
+  try (solve [eapply Crct_Sort; eassumption]).
+  - constructor.
+  - constructor.
+  - apply CrctWkTrmTrm; try assumption. eapply Crct_Sort; eassumption.
+  - apply CrctWkTrmTyp; try assumption. eapply Crct_Sort; eassumption.
 Qed.
 
 (** Tail preserves correctness **)
@@ -479,34 +384,76 @@ Qed.
 
 Lemma CrctTypTl:
   forall pp n t, Crct pp n t ->
-    forall nm npars tp p, pp = ((nm,ecTyp npars  tp)::p) -> CrctTyp p n tp.
+   forall nm npars tp p, pp = ((nm,ecTyp npars tp)::p) -> CrctTyp p n tp.
 induction 1; intros; try discriminate;
 try (solve [eapply IHCrct2; eassumption]);
-try (solve [eapply IHCrct; eassumption]);
-try (solve [eapply IHCrct1; eassumption]);
-try discriminate.
+try (solve [eapply IHCrct; eassumption]).
 - injection H2; intros. subst. assumption.
+- eapply IHCrct1. eassumption.
 Qed.
 
 
-(**
-Lemma CrctsWk: 
-  forall p n ts, Crcts p n ts -> forall s nm, Crct p n s ->
-           fresh nm p -> Crcts ((nm,ecTrm s)::p) n ts.
-induction 1; intros.
-- apply CrctsNil. apply CrctWk; assumption.
-- apply CrctsCons.
-  + apply CrctWk; assumption.
-  + apply IHCrcts; assumption.
-Qed.
+(******** different approach to correctness checking constructors  ***
+Inductive Crct: environ -> nat -> envClass -> Prop :=
+| CrctSrt: forall n, Crct nil n (ecTrm (TSort))
+| CrctWk: forall n p t s nm, Crct p n t -> Crct p n s ->
+           fresh nm p -> Crct ((nm,s)::p) n t
+| CrctRel: forall n m p, m < n -> Crct p 0 (ecTrm prop) ->
+                         Crct p n (ecTrm (TRel m))
+| CrctCast: forall n p t ck ty,
+              Crct p n (ecTrm t) -> Crct p n (ecTrm ty) ->
+              Crct p n (ecTrm (TCast t ck ty))
+| CrctProd: forall n p nm ty bod,
+              Crct p (S n) (ecTrm bod) -> Crct p n (ecTrm ty) ->
+              Crct p n (ecTrm (TProd nm ty bod))
+| CrctLam: forall n p nm ty bod,
+             Crct p (S n) (ecTrm bod) -> Crct p n (ecTrm ty) ->
+             Crct p n (ecTrm (TLambda nm ty bod))
+| CrctLetIn: forall n p nm dfn ty bod,
+         Crct p n (ecTrm dfn) -> Crct p (S n) (ecTrm bod) ->
+         Crct p n (ecTrm ty) -> 
+         Crct p n (ecTrm (TLetIn nm dfn ty bod))
+| CrctApp: forall n p fn a args,
+             Crct p n (ecTrm fn) -> Crct p n (ecTrm a) -> Crcts p n args -> 
+             Crct p n (ecTrm (TApp fn a args))
+| CrctConst: forall n p pd nm,
+               Crct p n (ecTrm prop) -> LookupDfn nm p pd ->
+               Crct p n (ecTrm (TConst nm))
+| CrctConstruct: forall n p i m1,
+                   Crct p n (ecTrm prop) -> Crct p n (ecTrm (TConstruct i m1))
+| CrctCase: forall n p m ty mch brs,
+              Crct p n (ecTrm mch) -> Crcts p n brs -> Crct p n (ecTrm ty) -> 
+              Crct p n (ecTrm (TCase m ty mch brs))
+| CrctFix: forall n p ds m, CrctDs p (n + dlength ds) ds ->
+                            Crct p n (ecTrm (TFix ds m))
+with Crcts: environ -> nat -> Terms -> Prop :=
+| CrctsNil: forall n p, Crct p n (ecTrm prop) -> Crcts p n tnil
+| CrctsCons: forall n p t ts,
+               Crct p n (ecTrm t) -> Crcts p n ts -> Crcts p n (tcons t ts)
+with CrctDs: environ -> nat -> Defs -> Prop :=
+| CrctDsNil: forall n p, Crct p n (ecTrm prop) -> CrctDs p n dnil
+| CrctDsCons: forall n p dn dty db dra ds,
+          Crct p n (ecTrm dty) -> Crct p n (ecTrm db) -> CrctDs p n ds ->
+          CrctDs p n (dcons dn dty db dra ds)
+with CrctTyp: environ -> nat -> itypPack -> Prop := 
+| CrctTypStart: forall p n itp, Crct p n (ecTrm prop) -> CrctTyp p n itp.
+Hint Constructors Crct Crcts CrctDs CrctTyp.
+Scheme Crct_ind' := Minimality for Crct Sort Prop
+  with Crcts_ind' := Minimality for Crcts Sort Prop
+  with CrctDs_ind' := Minimality for CrctDs Sort Prop
+  with CrctTyp_ind' := Minimality for CrctTyp Sort Prop.
+Combined Scheme CrctCrctsCrctDsTyp_ind from
+         Crct_ind', Crcts_ind', CrctDs_ind', CrctTyp_ind'.
+
 
 Lemma Crct_WFTrm:
-  (forall p n t, Crct p n t -> WFTrm t n) /\
+  (forall p n ec, Crct p n ec -> forall t, ec = ecTrm t -> WFTrm t n) /\
   (forall p n ts, Crcts p n ts -> WFTrms ts n) /\
-  (forall (p:environ) (n:nat) (ds:Defs), CrctDs p n ds -> WFTrmDs ds n).
-apply CrctCrctsCrctDs_ind; intros; auto; subst.
+  (forall (p:environ) (n:nat) (ds:Defs), CrctDs p n ds -> WFTrmDs ds n) /\
+  (forall (p:environ) (n:nat) (itp:itypPack), CrctTyp p n itp -> True).
+apply CrctCrctsCrctDsTyp_ind; intros; auto;
 Qed.
-**)
+*****************)
 
 Lemma Crct_fresh_Pocc:
   (forall p n t, Crct p n t -> forall nm, fresh nm p -> ~ PoccTrm nm t) /\
@@ -521,12 +468,17 @@ try (solve [inversion_clear j; elim (H0 nm); trivial; elim (H2 nm); trivial]);
 try (solve [inversion_clear j; elim (H0 nm0); trivial; elim (H2 nm0); trivial]);
 try (solve [inversion_clear j; elim (H0 nm); trivial; elim (H2 nm); trivial]);
 try (solve [inversion_clear H4; elim (H0 nm0); trivial]).
-- inversion_clear j; elim (H1 nm); trivial. elim (H3 nm); trivial.
-  elim (H5 nm); trivial.
+- inversion_clear j; elim (H0 nm0); trivial. elim (H2 nm0); trivial.
+  elim (H4 nm0); trivial.
+- inversion_clear j. elim (H1 nm); trivial. elim (H3 nm); trivial.
+  induction args. inversion H7. elim (H5 nm); trivial.
 - inversion j. subst. elim (@fresh_Lookup_fails _ _ (ecTrm pd) H2). assumption.
 - inversion_Clear j. eelim (fresh_Lookup_fails H3). eassumption.
+- inversion_Clear j. elim (H0 nm); trivial. elim (H2 nm); trivial.
+  elim (H4 nm); trivial.
+- inversion_clear j. elim (H0 nm); trivial. elim (H2 nm); trivial.
+  elim (H4 nm); trivial.
 Qed.
-
 
 Lemma Crct_not_bad_Lookup:
   (forall p n s, Crct p n s ->
@@ -540,11 +492,11 @@ apply CrctCrctsCrctDsTyp_ind; intros; auto;
 try (solve [elim (H0 _ H3)]); try (solve [elim (H0 _ H5)]);
 try (solve [elim (H0 _ H1)]); try (solve [elim (H0 _ H2)]).
 - inversion H.
-- inversion H.
+- cbv in H. inversion H.
 - destruct (string_dec nm0 nm).
   + subst. inversion_Clear H4.
     * assert (j:= proj1 Crct_fresh_Pocc _ _ _ H1 _ H3).
-      elim j. constructor.
+      elim j. constructor. 
     * elim (H0 _ H11).
   + eelim (H0 _ (Lookup_strengthen H4 _ n0)).
 - elim (H0 nm0). unfold LookupDfn in H4. unfold LookupDfn.
@@ -556,6 +508,7 @@ try (solve [elim (H0 _ H1)]); try (solve [elim (H0 _ H2)]).
 Grab Existential Variables.
   + reflexivity.
 Qed.
+
 
 Lemma  Crct_weaken:
   (forall p n t, Crct p n t -> 
@@ -572,7 +525,6 @@ eapply CrctCrctsCrctDsTyp_ind; intros; intuition.
   apply H0; try assumption. apply Lookup_weaken; eassumption.
 Qed.
 
-
 Lemma  Crct_Typ_weaken:
   (forall p n t, Crct p n t -> 
     forall nm itp, fresh nm p -> CrctTyp p n itp ->
@@ -585,7 +537,7 @@ Lemma  Crct_Typ_weaken:
                    forall npars, CrctDs ((nm,ecTyp npars itp)::p) n ds) /\
   (forall p n jtp, CrctTyp p n jtp -> 
     forall nm itp, fresh nm p -> CrctTyp p n itp ->
-                   forall npars, CrctTyp ((nm,ecTyp npars itp)::p) n jtp).
+                  forall npars,  CrctTyp ((nm,ecTyp npars itp)::p) n jtp).
 Proof.
   eapply CrctCrctsCrctDsTyp_ind; intros; auto.
   - apply CrctWkTrmTyp; try assumption. eapply CrctConst; try eassumption.
@@ -594,15 +546,15 @@ Proof.
 Qed.
 
 Lemma Crct_strengthen:
-  (forall pp n s, Crct pp n s -> forall nm ec p, pp = (nm,ec)::p ->
-                 ~ PoccTrm nm s -> Crct p n s) /\
-  (forall pp n ss, Crcts pp n ss -> forall nm ec p, pp = (nm,ec)::p ->
-                 ~ PoccTrms nm ss -> Crcts p n ss) /\
-  (forall pp n ds, CrctDs pp n ds -> forall nm ec p, pp = (nm,ec)::p ->
-                 ~ PoccDefs nm ds -> CrctDs p n ds) /\
-  (forall (pp:environ) (n:nat) (itp:itypPack), CrctTyp pp n itp -> True).
-apply CrctCrctsCrctDsTyp_ind; intros; auto.
-- discriminate.
+  (forall pp n t, Crct pp n t -> 
+       forall nm ec p, pp = (nm,ec)::p -> ~ PoccTrm nm t -> Crct p n t) /\
+  (forall pp n ts, Crcts pp n ts -> 
+       forall nm ec p, pp = (nm,ec)::p -> ~ PoccTrms nm ts -> Crcts p n ts) /\
+  (forall pp n ds, CrctDs pp n ds -> 
+       forall nm ec p, pp = (nm,ec)::p -> ~ PoccDefs nm ds -> CrctDs p n ds) /\
+  (forall p n itp, CrctTyp p n itp -> True).
+eapply CrctCrctsCrctDsTyp_ind; intros; auto.
+- inversion H.
 - discriminate.
 - injection H4; intros. subst. assumption.
 - injection H4; intros. subst. assumption.
@@ -610,22 +562,26 @@ apply CrctCrctsCrctDsTyp_ind; intros; auto.
   intros h. inversion h.
 - apply CrctCast.
   + eapply H0. eassumption.
-    intros h. elim H2. apply PoCast. assumption.
+    intros h. elim H4. apply PoCastTm. assumption.
+  + eapply H2. eassumption.
+    intros h. elim H4. apply PoCastTy. assumption.
 - apply CrctProd.
   + eapply H0. eassumption.
-    intros h. inversion h.
-  + eapply H2. eassumption.
     intros h. elim H4. apply PoProdBod. assumption.
+  + eapply H2. eassumption.
+    intros h. elim H4. apply PoProdTy. assumption.
 - apply CrctLam.
   + eapply H0. eassumption.
-    intros h. inversion h.
-  + eapply H2. eassumption.
     intros h. elim H4. apply PoLambdaBod. assumption.
+  + eapply H2. eassumption.
+    intros h. elim H4. apply PoLambdaTy. assumption.
 - apply CrctLetIn.
   + eapply H0. eassumption.
-    intros h. elim H4. apply PoLetInDfn. assumption.
+    intros h. elim H6. apply PoLetInDfn. assumption.
   + eapply H2. eassumption.
-    intros h. elim H4. apply PoLetInBod. assumption.
+    intros h. elim H6. apply PoLetInBod. assumption.
+  + eapply H4. eassumption.
+    intros h. elim H6. apply PoLetInTy. assumption.
 - apply CrctApp. assumption.
   + eapply H1. eassumption.
     intros h. elim H7. apply PoAppL. assumption.
@@ -634,9 +590,12 @@ apply CrctCrctsCrctDsTyp_ind; intros; auto.
   + eapply H5. eassumption.
     intros h. elim H7. apply PoAppR. assumption.
 - eapply CrctConst. eapply H0. eapply H2.
-  + intros h. inversion h.
-  + unfold LookupDfn in *. refine (Lookup_strengthen H1 H2 _).
-    apply neq_sym. apply notPocc_TConst. assumption.
+    intros h. inversion h. rewrite H2 in H1.
+    assert (j: nm0 <> nm).
+    { apply notPocc_TConst. assumption. }
+    inversion H1.
+  + rewrite H6 in j. nreflexivity j.
+  + eassumption.
 - eapply CrctConstruct; try eassumption.
   + eapply H0. eapply H3. intros h. inversion h.
   + rewrite H3 in H1.
@@ -647,9 +606,11 @@ apply CrctCrctsCrctDsTyp_ind; intros; auto.
     * eassumption.
 - apply CrctCase.
   + eapply H0. eassumption.
-    intros h. elim H4. apply PoCaseL. assumption.
+    intros h. elim H6. apply PoCaseL. assumption.
   + eapply H2. eassumption.
-    intros h. elim H4. apply PoCaseR. assumption.
+    intros h. elim H6. apply PoCaseR. assumption.
+  + eapply H4. eassumption.
+    intros h. elim H6. apply PoCaseTy. assumption.
 - apply CrctFix.
   + eapply H0. eassumption. intros h. inversion h.
   + eapply H2. eassumption. intros h. elim H4. apply PoFix. assumption.
@@ -661,8 +622,9 @@ apply CrctCrctsCrctDsTyp_ind; intros; auto.
     intros h. elim H4. apply PoTtl. assumption.
 - apply CrctDsNil. eapply H0. eassumption. intros h. inversion h.
 - apply CrctDsCons.
-  + eapply H0. eassumption. intros h. elim H4. apply PoDhd_bod. assumption.
-  + eapply H2. eassumption. intros h. elim H4. apply PoDtl. assumption.
+  + eapply H0. eassumption. intros h. elim H6. apply PoDhd_ty. assumption.
+  + eapply H2. eassumption. intros h. elim H6. apply PoDhd_bod. assumption.
+  + eapply H4. eassumption. intros h. elim H6. apply PoDtl. assumption.
 Qed.
 
 (** Crct inversions **)
@@ -680,7 +642,7 @@ assert (lem: (forall p n t, Crct p n t ->
     try (solve [eapply H2; eassumption]);
     try (solve [eapply H0; eassumption]).
     - inversion H.
-    - inversion H.
+    - inversion H. 
     - apply CrctWkTrmTrm; try assumption. inversion H4; subst.
       + assumption.
       + eapply H0. apply H11.
@@ -689,7 +651,6 @@ assert (lem: (forall p n t, Crct p n t ->
   }
   apply (proj1 lem).
 Qed.
-
 
 Lemma Crct_invrt_Rel:
   forall p n rel, Crct p n rel -> forall m, rel = TRel m ->
@@ -734,51 +695,53 @@ Proof.
         - assumption. }
       apply (LMiss _ j). trivial.
     + apply CrctWkTrmTyp; trivial.
-  - myInjection H1. intuition. exists pd; intuition.
+  - injection H1. intros. subst. intuition. exists pd; intuition.
     eapply LookupDfn_pres_Crct; eassumption.
 Qed.
 
 Lemma Crct_invrt_Prod:
   forall p n prod, Crct p n prod ->
-  forall nm bod, prod = TProd nm bod -> Crct p (S n) bod.
-Proof.
-  induction 1; intros; try discriminate.
-  - assert (j:= IHCrct1 _ _ H2).
-    apply CrctWkTrmTrm; trivial.
-    apply (proj1 Crct_up). assumption.
-  - assert (j:= IHCrct _ _ H2).
-    apply CrctWkTrmTyp; trivial.
-    apply (proj2 (proj2 (Crct_up))). assumption.    
-  - injection H1. intros. subst. assumption.
-Qed.
-
-Lemma Crct_invrt_Lam:
-  forall p n lam, Crct p n lam ->
-  forall nm bod, lam = TLambda nm bod -> Crct p (S n) bod.
-Proof.
-  induction 1; intros; try discriminate.
-  - assert (j:= IHCrct1 _ _ H2).
-    apply CrctWkTrmTrm; trivial.
-    apply (proj1 Crct_up). assumption.
-  - assert (j:= IHCrct _ _ H2).
-    apply CrctWkTrmTyp; trivial.
-    apply (proj2 (proj2 (Crct_up))). assumption.    
-  - injection H1. intros. subst. assumption.
-Qed.
-
-Lemma Crct_invrt_LetIn:
-  forall p n letin, Crct p n letin ->
-  forall nm dfn bod, letin = TLetIn nm dfn bod ->
-     Crct p n dfn /\ Crct p (S n) bod.
+  forall nm ty bod, prod = TProd nm ty bod ->
+     Crct p n ty /\ Crct p (S n) bod.
 Proof.
   induction 1; intros; try discriminate.
   - assert (j:= IHCrct1 _ _ _ H2). intuition.
     apply CrctWkTrmTrm; trivial.
     apply (proj1 (Crct_up)). assumption.
   - assert (j:= IHCrct _ _ _ H2). intuition.
+    apply (CrctWkTrmTyp);trivial.
+    apply (proj2 (proj2 (Crct_up))). assumption.    
+  - injection H1. intros. subst. intuition.
+Qed.
+
+Lemma Crct_invrt_Lam:
+  forall p n lam, Crct p n lam ->
+  forall nm ty bod, lam = TLambda nm ty bod ->
+     Crct p n ty /\ Crct p (S n) bod.
+Proof.
+  induction 1; intros; try discriminate.
+  - assert (j:= IHCrct1 _ _ _ H2). intuition.
+    apply CrctWkTrmTrm; trivial.
+    apply (proj1 (Crct_up)). assumption.
+  - assert (j:= IHCrct _ _ _ H2). intuition.
+    apply (CrctWkTrmTyp);trivial.
+    apply (proj2 (proj2 (Crct_up))). assumption.    
+  - injection H1. intros. subst. intuition.
+Qed.
+
+Lemma Crct_invrt_LetIn:
+  forall p n letin, Crct p n letin ->
+  forall nm dfn ty bod, letin = TLetIn nm dfn ty bod ->
+     Crct p n dfn /\ Crct p n ty /\ Crct p (S n) bod.
+Proof.
+  induction 1; intros; try discriminate.
+  - assert (j:= IHCrct1 _ _ _ _ H2). intuition.
+    apply CrctWkTrmTrm; trivial.
+    apply (proj1 (Crct_up)). assumption.
+  - assert (j:= IHCrct _ _ _ _ H2). intuition.
     apply (CrctWkTrmTyp); trivial.
     apply (proj2 (proj2 Crct_up)). assumption.
-  - injection H1. intros. subst. intuition.
+  - injection H2. intros. subst. intuition.
 Qed.
 
 Lemma Crct_invrt_App:
@@ -795,23 +758,24 @@ Qed.
 
 Lemma Crct_invrt_Case:
   forall p n case,
-    Crct p n case -> forall m s us, case = (TCase m s us) ->
-    Crct p n s /\ Crcts p n us.
+    Crct p n case -> forall m t s us, case = (TCase m t s us) ->
+    Crct p n t /\ Crct p n s /\ Crcts p n us.
 induction 1; intros; try discriminate.
-- assert (j:= IHCrct1 _ _ _ H2). intuition.
+- assert (j:= IHCrct1 _ _ _ _ H2). intuition.
   apply (proj2 Crct_weaken); auto.
-- assert (j:= IHCrct _ _ _ H2). intuition.
+- assert (j:= IHCrct _ _ _ _ H2). intuition.
   apply (proj1 (proj2 Crct_Typ_weaken)); auto.
-- injection H1; intros; subst. auto.
+- injection H2; intros; subst. auto.
 Qed.
 
 Lemma Crct_invrt_Cast:
   forall p n cast,
-    Crct p n cast -> forall t, cast = (TCast t) -> Crct p n t.
+    Crct p n cast -> forall t ck ty, cast = (TCast t ck ty) ->
+    Crct p n t /\ Crct p n ty.
 induction 1; intros; try discriminate.
-- assert (j:= IHCrct1 _ H2). intuition.
-- assert (j:= IHCrct _ H2). intuition.
-- injection H0; intros; subst. auto.
+- assert (j:= IHCrct1 _ _ _ H2). intuition.
+- assert (j:= IHCrct _ _ _ H2). intuition.
+- injection H1; intros; subst. auto.
 Qed.
 
 Lemma Crct_invrt_Fix:
@@ -830,11 +794,10 @@ induction 1; intros; try discriminate.
     * rewrite <- plus_n_Sm. apply Crct_up. assumption.
 - injection H1; intros; subst. assumption.
 Qed.
-
+  
 Lemma Crct_invrt_Construct:
   forall p n construct, Crct p n construct ->
-  forall ipkgNm inum cnum,
-    construct = (TConstruct (mkInd ipkgNm inum) cnum) ->
+  forall ipkgNm inum cnum, construct = (TConstruct (mkInd ipkgNm inum) cnum) ->
     Crct p n prop /\
     exists npars itypk,
       LookupTyp ipkgNm p npars itypk /\ CrctCnstr itypk inum cnum.
@@ -848,6 +811,13 @@ induction 1; intros; try discriminate.
 - injection H2; intros; subst. intuition.
   exists npars, itypk. intuition.
 Qed.
+
+Lemma Crct_invrt_any:
+  forall p n t, Crct p n t -> Crct p n prop.
+Proof.
+  induction 1; try (solve[constructor; eassumption]); try assumption.
+Qed.
+
 
 Lemma Crct_App_fn_notApp:
   forall p n fn arg args, Crct p n (TApp fn arg args) -> ~(isApp fn).
@@ -870,7 +840,7 @@ Lemma mkApp_pres_Crct:
   forall fn p n, Crct p n fn ->
   forall args, Crcts p n args -> Crct p n (mkApp fn args).
 Proof.
-  induction fn; unfold mkApp; simpl; intros p' nx h0 args h1;
+  induction fn; simpl; intros p' nx h0 args h1;
   destruct args; intuition;
   try (solve [inversion_Clear h1; apply CrctApp; try assumption; not_isApp]).
   - destruct (Crct_invrt_App h0 eq_refl) as [j1 [j2 [j3 j4]]].
@@ -892,29 +862,28 @@ Lemma Instantiate_pres_Crct:
   (forall n ds ids, InstantiateDefs tin n ds ids ->
   forall m p, n <= m -> CrctDs p (S m) ds -> Crct p m tin -> CrctDs p m ids).
 Proof.
-  intros tin. apply InstInstsDefs_ind; intros; trivial.
-  - destruct (Crct_invrt_Rel H0 eq_refl).
-    erewrite Crct_mkApp_ident; eassumption.
-  - apply CrctRel.
-    + omega.
-    + eapply Crct_Sort. eassumption.
+  intros tin. apply InstInstsDefs_ind; intros.
+  - assumption.
+  - constructor. omega. eapply Crct_invrt_any. eassumption.
   - destruct (Crct_invrt_Rel H0 eq_refl). apply CrctRel.
     + omega.
     + eapply Crct_Sort. eassumption.
   - eapply Crct_Sort; eassumption.
   - eapply Crct_Prf; eassumption.
-  - assert (j:= Crct_invrt_Cast H1 eq_refl). apply CrctCast.
-    apply H; trivial.
-  - apply CrctProd. eapply Crct_Sort; eassumption.
-    assert (j:= Crct_invrt_Prod H1 eq_refl).
+  - destruct (Crct_invrt_Cast H2 eq_refl). apply CrctCast.
+    + apply H; trivial.
+    + apply H0; trivial.
+  - destruct (Crct_invrt_Prod H2 eq_refl). apply CrctProd.
     + apply H; trivial. omega. apply (proj1 Crct_up). assumption.
-  -  apply CrctLam. eapply Crct_Sort; eassumption.
-     assert (j:= Crct_invrt_Lam H1 eq_refl).
+    + apply H0; trivial.
+  - destruct (Crct_invrt_Lam H2 eq_refl). apply CrctLam.
     + apply H; trivial. omega. apply (proj1 Crct_up). assumption.
-  - destruct (Crct_invrt_LetIn H2 eq_refl). apply CrctLetIn.
+    + apply H0; trivial.
+  - destruct (Crct_invrt_LetIn H3 eq_refl). apply CrctLetIn.
     + apply H; trivial.
     + apply H0; intuition. apply (proj1 Crct_up). assumption.
-  - destruct (Crct_invrt_App H3 eq_refl) as [j1 [j2 [j3 j4]]].
+    + apply H1; intuition.
+  - destruct (Crct_invrt_App H3 eq_refl) as [j1 [j2 [j3 j4]]]. 
     apply mkApp_pres_Crct.
     + apply H; trivial.
     + apply CrctsCons.
@@ -923,14 +892,15 @@ Proof.
   - edestruct (Crct_invrt_Const H0).
     + reflexivity.
     + destruct H3 as [x [h1 h2]]. eapply (@CrctConst _ _ x); trivial.
-      eapply Crct_Sort. eassumption.
+      * eapply Crct_Sort. eassumption.
   - apply CrctInd. eapply Crct_Sort. eassumption.
   - destruct ind. edestruct (Crct_invrt_Construct H0).
     + reflexivity.
     + destruct H3 as [npars [x [h1 h2]]]. eapply CrctConstruct; try eassumption.
       * eapply Crct_Sort. eassumption.
-  - destruct (Crct_invrt_Case H2 eq_refl) as [h1 h2]. apply CrctCase.
+  - destruct (Crct_invrt_Case H3 eq_refl) as [h1 [h2 h3]]. apply CrctCase.
     + apply H; trivial.
+    + apply H1; trivial.
     + apply H0; trivial.
   - assert (j:= Crct_invrt_Fix H1 eq_refl). apply CrctFix. 
     + eapply Crct_Sort. eassumption.
@@ -944,43 +914,82 @@ Proof.
     + apply H; trivial.
     + apply H0; trivial.
   - apply CrctDsNil. eapply Crct_Sort. eassumption.
-  - inversion_Clear H2. apply CrctDsCons.
+  - inversion_Clear H3. apply CrctDsCons.
     + apply H; trivial.
     + apply H0; trivial.
+    + apply H1; trivial.
 Qed.
 
-(***
-Lemma Crct_App_inv:
-  forall p n fn a1 args, Crct p n (TApp fn a1 args) ->
-                         Crct p n fn /\ Crct p n a1 /\ Crcts p n args.
-intros p n fn a1 args h. split; try split. inversion_Clear h.
-- inversion H; subst.
-induction 1. try (intros; discriminate); intros h; subst; split; try split;
-try (inversion_Clear h; assumption).
-- eapply CrctWkTrmTrm; try eassumption. intuition.
-- eapply CrctWkTrmTrm; try eassumption. intuition.
-- assert (j:Crct p n fn /\ Crct p n a1 /\ Crcts p n args).
-  apply IHCrct1; reflexivity.
-  destruct j. destruct H3.
-  eapply (CrctsWk H4); assumption. 
+Lemma instantiate_pres_Crct:
+  forall p m bod, Crct p (S m) bod ->
+  forall n tin, n <= m -> Crct p m tin -> Crct p m (instantiate tin n bod).
+Proof.
+  intros. eapply (proj1 (Instantiate_pres_Crct tin)); try eassumption.
+  - apply (proj1 (instantiate_Instantiate tin)). 
 Qed.
 
-Lemma Crct_App_inv:
-  forall p n fn a1 args t, Crct p n t -> t = (TApp fn a1 args) ->
-                         Crct p n fn /\ Crct p n a1 /\ Crcts p n args.
-intros p n fn a1 args t h j. 
-induction h; try (intros; discriminate). intros h. subst; split; try split;
-try (inversion_Clear h; assumption).
-- eapply CrctWkTrmTrm; try eassumption. intuition.
-- eapply CrctWkTrmTrm; try eassumption. intuition.
-- assert (j:Crct p n fn /\ Crct p n a1 /\ Crcts p n args).
-  apply IHCrct1; reflexivity.
-  destruct j. destruct H3.
-  eapply (CrctsWk H4); assumption. 
+Lemma whBetaStep_pres_Crct:
+  forall p n bod, Crct p (S n) bod ->
+  forall arg, Crct p n arg ->
+  forall args, Crcts p n args -> Crct p n (whBetaStep bod arg args).
+Proof.
+  intros. unfold whBetaStep. apply mkApp_pres_Crct; trivial.
+  + apply instantiate_pres_Crct; trivial. omega.
 Qed.
-***)
 
-(*********
+
+Lemma tnth_pres_Crct:
+  forall p n ts, Crcts p n ts ->
+  forall m s, tnth m ts = Some s -> Crct p n s.
+Proof.
+  induction 1; induction m; intros.
+  - simpl in H0. discriminate.
+  - simpl in H0. discriminate.
+  - simpl in H1. injection H1. intros. subst. assumption.
+  - simpl in H1. eapply IHCrcts. eassumption.
+Qed.
+
+Lemma tskipn_pres_Crct:
+  forall m ts ss, tskipn m ts = Some ss -> forall p n, Crcts p n ts ->
+  Crcts p n ss.
+Proof.
+induction m; induction ts; intros.
+- simpl in H. injection H; intros; subst. assumption.
+- simpl in H. injection H; intros; subst. assumption.
+- simpl in H. discriminate.
+- simpl in H. eapply IHm. eassumption. inversion H0. assumption.
+Qed.
+
+Lemma whCaseStep_pres_Crct:
+  forall p n ts, Crcts p n ts -> forall brs, Crcts p n brs ->
+  forall m s, whCaseStep m ts brs = Some s -> Crct p n s.
+Proof.
+  intros p n ts h1 brs h2 m s h3. unfold whCaseStep in h3.
+  assert (j: tnth m brs = None \/ (exists t, tnth m brs = Some t)).
+  { destruct (tnth m brs).
+    + right. exists t. reflexivity.
+    + left. reflexivity. }
+  destruct j.
+  - rewrite H in h3. discriminate.
+  - destruct H. rewrite H in h3. injection h3; intros. rewrite <- H0.
+    apply mkApp_pres_Crct; try assumption.
+    apply (tnth_pres_Crct h2 _ H).
+Qed. 
+
+Lemma fold_left_pres_Crct:
+  forall p m (f:Term -> nat -> Term) (ns:list nat) (t:Term),
+    (forall u, Crct p m u -> forall n, Crct p m (f u n)) ->
+    Crct p m t -> Crct p m (fold_left f ns t).
+Proof.
+  intros p n f. induction ns; simpl; intros.
+  - assumption.
+  - apply IHns.
+    + intros. apply H. assumption.
+    + apply H. assumption.
+Qed.
+
+
+(***********************
 (** An alternative correctness specification for programs: [crct], below **)
 Definition weaklyClosed (t:Term) (p:environ) : Prop :=
   forall nm, PoccTrm nm t -> lookupDfn nm p <> None.
@@ -992,13 +1001,55 @@ Fixpoint weaklyCloseds (ts:Terms) p : Prop :=
 Fixpoint weaklyClosedd (ds:Defs) p : Prop :=
   match ds with
     | dnil => True
-    | dcons nm tb m es => weaklyClosed tb p /\ weaklyClosedd es p
+    | dcons nm ty tb m es =>
+      weaklyClosed ty p /\ weaklyClosed tb p /\ weaklyClosedd es p
   end.
 
+(****  ???????
+Lemma Pocc_notWC:
+  forall nm,
+  (forall t, PoccTrm nm t -> ~ weaklyClosed t nil) /\
+  (forall ts, PoccTrms nm ts -> ~ weaklyCloseds ts nil) /\
+  (forall ds, PoccDefs nm ds -> ~ weaklyClosedd ds nil).
+intros nm; apply poTrmTrmsDefs_ind; unfold not; intros;
+           try (unfold weaklyClosed in H0; simpl in H0);
+           try (unfold weaklyClosed in H1; simpl in H1); 
+           try (apply H0; intros xnm h; apply (H1 xnm));
+           try (solve [constructor; assumption]).
+- apply PoCastTy. assumption.
+- apply PoProdTy. assumption.
+- apply PoLambdaTy. assumption.
+- apply PoLetInBod; assumption.
+- apply PoLetInTy; assumption.
+- apply PoAppA. assumption.
+- apply H0. elim (H1 nm); auto. apply PoAppR. assumption.
+- elim (H0 nm); auto. constructor. assumption.
+- elim (H1 nm); auto. apply PoCaseR. assumption.
+- elim (H1 nm); auto. apply PoCaseTy. assumption.
+- elim (H1 nm); auto. apply PoFix. assumption.
+- destruct H1. apply H0. intros xnm h. unfold weaklyClosed in H1.
+  apply (H1 nm). assumption.
+- destruct H1. apply H0. assumption.
+- destruct H1. apply H0. intros nm0 j. induction ds.
+  elim H0.
+
+  apply (H2 nm). assumption.
+- intuition.
+Qed.
+**************)
+
+Lemma weaklyClosed_TCast:
+  forall t ty c p, weaklyClosed (TCast t c ty) p ->
+                   weaklyClosed t p /\ weaklyClosed ty p.
+unfold weaklyClosed. intros t ty c pb h1. split; intros nm h2.
+- apply h1. apply PoCastTm. assumption.
+- apply h1. apply PoCastTy. assumption.
+Qed.
+
 Lemma weaklyClosed_TCase:
-  forall n mch brs p, weaklyClosed (TCase n mch brs) p ->
-            weaklyClosed mch p /\ weaklyCloseds brs p.
-unfold weaklyClosed. intros n mch brs p h1. split.
+  forall n ty mch brs p, weaklyClosed (TCase n ty mch brs) p ->
+            weaklyClosed mch p /\ weaklyCloseds brs p /\ weaklyClosed ty p.
+unfold weaklyClosed. intros n ty mch brs p h1. split; [|split].
 - intros xnm h2. apply (h1 xnm). apply PoCaseL. assumption.
 - induction brs; unfold weaklyCloseds. auto. split.
   + unfold weaklyClosed. intros xnm h2. apply (h1 xnm).
@@ -1006,6 +1057,8 @@ unfold weaklyClosed. intros n mch brs p h1. split.
   + apply IHbrs. intros xnm h2. apply (h1 xnm). inversion_clear h2.
     apply PoCaseL. assumption.
     apply PoCaseR. apply PoTtl. assumption.
+    apply PoCaseTy. assumption.
+- intros xnm h2. apply (h1 xnm). apply PoCaseTy. assumption.
 Qed.
 
 Lemma Pocc_weakClsd_no_lookup:
@@ -1013,10 +1066,15 @@ Lemma Pocc_weakClsd_no_lookup:
                forall p, weaklyClosed t p -> lookupDfn nm p <> None.
 induction 1; intros p h1; unfold weaklyClosed in h1; apply h1;
 try (solve [constructor; assumption]).
+- apply PoCastTy. assumption.
+- apply PoProdTy. assumption.
+- apply PoLambdaTy. assumption.
 - apply PoLetInBod. assumption.
+- apply PoLetInTy. assumption.
 - apply PoAppA. assumption.
 - apply PoAppR. assumption.
 - apply PoCaseR. assumption.
+- apply PoCaseTy. assumption.
 Qed.
 
 Lemma weaklyClosed_weaken:
@@ -1082,7 +1140,7 @@ induction 1; intros; intros h.
   reflexivity.
 Qed.
 
-(*********************** ??????
+(******************  ????????????
 Lemma Crct_weaklyClosed:
   (forall p n t, Crct p n t -> weaklyClosed t p) /\
   (forall p n ts, Crcts p n ts -> weaklyCloseds ts p) /\
@@ -1092,12 +1150,16 @@ try (solve [inversion H|inversion H0|simpl;auto]).
 - destruct (string_dec nm0 nm); unfold lookupDfn.
   + subst. rewrite (string_eq_bool_rfl nm). intros j. discriminate.
   + rewrite (string_eq_bool_neq n0). apply H0. assumption.
-- inversion_clear H2.
-- inversion_clear H1. apply H0. assumption.
-- inversion_clear H1. apply H0. assumption.
+- inversion_clear H2. 
+- inversion_clear H3. apply H0. assumption. apply H2. assumption.
+- inversion_clear H3. apply H0. assumption. apply H2. assumption.
 - inversion_clear H3.
   + apply H0. assumption.
   + apply H2. assumption.
+- inversion_clear H5.
+  + apply H0. assumption.
+  + apply H2. assumption.
+  + apply H4. assumption.
 - inversion_clear H5. 
   + apply H0. assumption.
   + apply H2. assumption.
@@ -1105,17 +1167,21 @@ try (solve [inversion H|inversion H0|simpl;auto]).
     * inversion_clear H6. destruct H4. unfold weaklyClosed in H4.
       apply (H4 nm H5). destruct H4. inversion_clear H3.
       apply IHargs; assumption.
-- inversion H2. rewrite (string_eq_bool_eq _ _ H4). assumption.
+- inversion H2. rewrite (string_eq_bool_eq _ _ H4). intros h. 
+  assert (j:= @lookupDfn_None_not_LookupDfn _ _ pd h). contradiction.
 - inversion H1.
-- inversion_clear H3. 
-  + apply (H0 nm). assumption.
-  + induction brs; destruct H2; inversion_clear H4.
-    * unfold weaklyClosed in H2. apply (H2 nm). assumption.
+- inversion_clear H5.
+  + apply H0. assumption.
+  + induction brs; destruct H2; inversion_clear H6. 
+    * unfold weaklyClosed in H2. apply H2. assumption.
     * inversion_clear H1. eapply IHbrs; assumption.
+  + apply H4. assumption.
 - inversion_clear H1.
-  induction ds; inversion_clear H2; inversion_clear H; destruct H0.
-  + unfold weaklyClosed in H. eapply H. assumption.
-  + apply IHds. simpl in H3. try assumption.
+  induction ds; inversion_clear H2; inversion_clear H;
+  destruct H0; destruct H0.
+  + unfold weaklyClosed in H. apply (H _ H1).
+  + unfold weaklyClosed in H0. apply (H0 _ H1).
+  + apply IHds; assumption.
 Qed.
 
 Lemma Crct_envOk:
@@ -1161,5 +1227,6 @@ unfold weaklyClosed; intros nmy h3; inversion_clear h3; simpl.
 - rewrite (string_eq_bool_eq _ _ H2). rewrite (string_eq_bool_neq H7). 
   rewrite (proj2 (lookupDfn_LookupDfn _ _ _) H8). intuition. discriminate.
 Qed.
-***************)
-***********************)
+
+**********************************)
+******************************************)
