theories/L3_flattenedApp/unaryApplications.v
@@ -1,12 +1,12 @@
 (******)
 Add LoadPath "../common" as Common.
 Add LoadPath "../L1_MalechaQuoted" as L1.
-Add LoadPath "../L2_typeStrippedL1" as L2.
+Add LoadPath "../L1_5_box" as L1_5.
+Add LoadPath "../L2_typeStripped" as L2.
 Add LoadPath "../L3_flattenedApp" as L3.
 (******)
 
-Require L2.L2.
-Require L1.L1.
+Require L2.compile.
 
 Require Import Coq.Lists.List.
 Require Import Coq.Strings.String.
@@ -19,225 +19,21 @@ Require Import L3.program.
 Require Import L3.wndEval.
 Require Import L3.wcbvEval.
 Require Import L3.wNorm.
+Require Import L3.compile.
 
 Local Open Scope string_scope.
 Local Open Scope bool.
 Local Open Scope list.
 Set Implicit Arguments.
 
-Definition L2Term := L2.term.Term.
-Definition L2Terms := L2.term.Terms.
-Definition L2Defs := L2.term.Defs.
-
-(** turn (App fn [x1;...;xn]) into (App (... (App fn x1) x2 ...) xn) **)
-Function mkApp (fn:Term) (xs:Terms) : Term :=
-    match xs with
-      | tnil => fn
-      | tcons b ys => mkApp (TApp fn b) ys
-    end.
-
-(** turn (Constructor [x1;...;xn; 0;...k]])  with arity n+k into
-*** (Lam ... (Lam (Const [x1;...;xn; 0;...k])...))
-**)
-Function mkEta (cstr:Term) (xtraArity:nat) : Term :=
-    match xtraArity with
-      | 0 => cstr
-      | S n => mkEta (TLambda nAnon cstr) n
-    end.
-
-Lemma mkEta_under_Lambda:
-  forall n t, mkEta (TLambda nAnon t) n = TLambda nAnon (mkEta t n).
-Proof.
-  induction n; simpl; intros.
-  - reflexivity.
-  - rewrite IHn. reflexivity.
-Qed.
-
-(** Lookup constructor arity in L2 environ (to avoid mutual dependency
-*** between converting L2 terms to L3 and L2 environs to L3)
-**)
-Section EtaExpand.
-Variable p:L2.program.environ.
-
-(** temp: here we assume the type of constructors is evaluated **)
-(** when removing this; also remove L2.program.arity_from_dtyp **)
-Function cnstrArity (i:inductive) (n:nat) : exception nat :=
-  match i with
-    | mkInd str m => L2.program.cnstrArity str m n p
-  end.
-
-(** compute list of variables for eta expanding a constructor
-*** (which may already be partially applied)
-**)
-Function etaArgs (n:nat) : Terms :=
-  match n with
-    | 0 => tnil
-    | S m => tcons (TRel m) (etaArgs m)
-  end.
-
-Function etaExp_cnstr (i:inductive) (n:nat) (args:Terms) : exception Term :=
-  match cnstrArity i n with
-    | Ret arity =>
-      match nat_compare (tlength args) arity with
-        | Eq => Ret (TConstruct i n args)
-        | Lt => let k := arity - (tlength args)
-                in Ret (mkEta (TConstruct i n (tappend args (etaArgs k))) k)
-        | Gt => Exc ("more arguments than constructor arity: "
-                       ++ (nat_to_string (tlength args)) ++ (" ")
-                       ++ (nat_to_string arity))
-      end
-    | Exc x => Exc x
-  end.
-
-Function strip (t:L2Term) : exception Term :=
-  match t with
-    | L2.term.TProof => Ret TProof
-    | L2.term.TRel n => Ret (TRel n)
-    | L2.term.TSort s => Ret (TSort s)
-    | L2.term.TCast s => strip s
-    | L2.term.TProd nm bod => 
-      match strip bod with
-        | Ret sbod => Ret (TProd nm sbod)
-        | x => x
-      end
-    | L2.term.TLambda nm bod =>
-      match strip bod with
-        | Ret sbod => Ret (TLambda nm sbod)
-        | x => x
-      end
-    | L2.term.TLetIn nm dfn bod => 
-      match strip dfn, strip bod with
-        | Ret sdfn, Ret sbod => Ret (TLetIn nm sdfn sbod)
-        | Exc s, Ret _ => Exc ("strip dfn fails:" ++ s)
-        | Ret _, Exc s => Exc ("strip bod fails:" ++ s)
-        | Exc s1, Exc s2 => Exc "both strip dfn and strip bod fail"
-      end
-    | L2.term.TApp fn arg args =>
-      match strip arg, strips args with
-        | Ret sarg, Ret sargs =>
-          match fn with 
-            | L2.term.TConstruct i n => etaExp_cnstr i n (tcons sarg sargs)
-            | x => match strip x with
-                     | Ret sx => Ret (mkApp sx (tcons sarg sargs))
-                     | x => x
-                   end
-          end
-        | Exc s, Ret _ => Exc ("strip arg fails:" ++ s)
-        | Ret _, Exc s => Exc ("strips args fails:" ++ s)
-        | Exc s1, Exc s2 => Exc "both strip arg and strips args fail"
-      end
-    | L2.term.TConst nm =>
-      match L2.program.lookup nm p with
-        | Some (L2.program.ecTrm _) => Ret (TConst nm)
-        | Some L2.program.ecAx => Ret (TAx nm)
-        | Some (L2.program.ecTyp _ _) =>
-          Exc "L2.program.lookup nm p returns a type"
-        | None => Exc "L2.program.lookup nm p misses"
-      end
-    | L2.term.TInd i => Ret (TInd i)
-    | L2.term.TConstruct i n => etaExp_cnstr i n tnil
-    | L2.term.TCase n mch brs =>
-      match strip mch, strips brs with
-        | Ret smch, Ret sbrs => Ret (TCase n smch sbrs)
-        | Exc s, Ret _ => Exc ("strip mch fails:" ++ s)
-        | Ret _, Exc s => Exc ("strips brs fails:" ++ s)
-        | Exc s1, Exc s2 => Exc "both strip mch and strips brs fail"
-      end
-    | L2.term.TFix ds n =>
-      match stripDs ds with
-        | Ret sds => Ret (TFix sds n)
-        | Exc s => Exc "stripDs ds fails"
-      end
-   end
-with strips (ts:L2Terms) : exception Terms := 
-  match ts with
-    | L2.term.tnil => Ret tnil
-    | L2.term.tcons t ts =>
-      match strip t, strips ts with
-        | Ret st, Ret sts => Ret (tcons st sts)
-        | Exc s, Ret _ => Exc ("strip t fails:" ++ s)
-        | Ret _, Exc s => Exc ("strips ts fails:" ++ s)
-        | Exc s1, Exc s2 => Exc "both strip t and strips ts fail"
-      end
-  end
-with stripDs (ts:L2Defs) : exception Defs := 
-  match ts with
-    | L2.term.dnil => Ret dnil
-    | L2.term.dcons nm t m ds =>
-      match strip t, stripDs ds with
-        | Ret st, Ret sds => Ret (dcons nm st m sds)
-        | Exc s, Ret _ => Exc ("strip t fails:" ++ s)
-        | Ret _, Exc s => Exc ("stripDs ds fails:" ++ s)
-        | Exc s1, Exc s2 => Exc "both strip t and stripDs ds fail"
-      end
-  end.
-(**
-Functional Scheme strip_ind' := Induction for strip Sort Prop
-with strips_ind' := Induction for strips Sort Prop
-with stripDs_ind' := Induction for stripDs Sort Prop.
-Combined Scheme stripStripsStripDs_ind
-         from strip_ind', strips_ind', stripDs_ind'.
-***)
-End EtaExpand.
-
-
-
-Function stripCnstrs (cs:list L2.program.Cnstr) : list Cnstr :=
-  match cs with
-    | nil => nil
-    | cons (L2.program.mkCnstr str arity) cs =>
-        cons (mkCnstr str arity) (stripCnstrs cs)
-  end.
-Function stripItyPack (its:L2.program.itypPack) : itypPack :=
-  match its with
-    | nil => nil
-    | (L2.program.mkItyp str itps) :: itpacks =>
-                  (mkItyp str (stripCnstrs itps)) :: stripItyPack itpacks
-  end.
-Function stripEnv (p:L2.program.environ) : exception environ :=
-  match p with
-    | nil => Ret nil
-    | cons (nm, L2.program.ecTrm t) q =>
-      match strip q t, stripEnv q with
-        | Ret ts, Ret qs => Ret (cons (nm, ecTrm ts) qs)
-        | Exc s, Ret _ => Exc ("strip q t fails:" ++ s)
-        | Ret _, Exc s => Exc ("stripEnv q fails:" ++ s)
-        | Exc s1, Exc s2 => Exc "both strip q t and stripEnv q fail"
-      end
-    | cons (nm, L2.program.ecTyp m ityps) q =>
-      match stripEnv q with
-        | Ret qs => Ret (cons (nm, ecTyp m (stripItyPack ityps)) qs)
-        | x => x
-      end
-    | cons (nm, L2.program.ecAx) q => stripEnv q
-  end.
-
-
-(** start-to-L3 translations **)
-Definition program_Program 
-           (e:L2.program.environ) (pgm:program) : exception Program :=
-  match L1.malecha_L1.program_Program pgm (Ret nil) with
-    | Ret pgm => 
-      match stripEnv (L2.stripEvalCommute.stripEnv (L1.program.env pgm)),
-            strip e (L2.stripEvalCommute.strip (L1.program.main pgm)) with
-        | Ret senv, Ret smain => Ret {| env:= senv; main:= smain |}
-        | Exc s, Ret _ => Exc ("program_Program: stripEnv fails:" ++ s)
-        | Ret _, Exc s => Exc ("program_Program: strip fails:" ++ s)
-        | Exc s1, Exc s2 =>
-          Exc "program_Program: both stripEnv and strip fail"
-      end
-    | Exc s => Exc s
-  end.
-Definition term_Term (e:L2.program.environ) (t:term) : exception Term :=
-  match L1.malecha_L1.term_Term t with
-    | Exc str => Exc str
-    | Ret trm => strip e (L2.stripEvalCommute.strip trm)
-  end.
+Definition L2Term := L2.compile.Term.
+Definition L2Terms := L2.compile.Terms.
+Definition L2Defs := L2.compile.Defs.
 
 
 Lemma strip_Lam_invrt:
   forall p nm bod tt,
-        strip p (L2.term.TLambda nm bod) = Ret tt ->
+        strip p (L2.compile.TLambda nm bod) = Ret tt ->
         exists sbod, strip p bod = Ret sbod /\ tt = TLambda nm sbod.
 Proof.
   induction tt; simpl; intros. 
@@ -277,7 +73,7 @@ Proof.
     destruct (strip p bod); discriminate.
   - change ((match strip p bod with
               | Ret sbod => Ret (TLambda nm sbod)
-              | Exc s => Exc s end) = Ret (TAx s)) in H.
+              | Exc s => Exc s end) = Ret TAx) in H.
     destruct (strip p bod); discriminate.    
   - change ((match strip p bod with
               | Ret sbod => Ret (TLambda nm sbod)
@@ -299,7 +95,7 @@ Qed.
 
 Lemma strip_Prod_invrt:
   forall p nm bod tt,
-        strip p (L2.term.TProd nm bod) = Ret tt ->
+        strip p (L2.compile.TProd nm bod) = Ret tt ->
         exists sbod, strip p bod = Ret sbod /\ tt = TProd nm sbod.
 Proof.
   induction tt; simpl; intros. 
@@ -339,7 +135,7 @@ Proof.
     destruct (strip p bod); discriminate.
   - change ((match strip p bod with
               | Ret sbod => Ret (TProd nm sbod)
-              | Exc s => Exc s end) = Ret (TAx s)) in H.
+              | Exc s => Exc s end) = Ret TAx) in H.
     destruct (strip p bod); discriminate.
   - change ((match strip p bod with
               | Ret sbod => Ret (TProd nm sbod)
@@ -361,7 +157,7 @@ Qed.
 
 Lemma strip_Construct_invrt:
   forall p i r tt,
-        strip p (L2.term.TConstruct i r) = Ret tt ->
+        strip p (L2.compile.TConstruct i r) = Ret tt ->
         etaExp_cnstr p i r tnil = Ret tt.
 Proof.
   induction tt; unfold strip; simpl; intros; try assumption.
@@ -369,7 +165,7 @@ Qed.
  
 Lemma strip_Ind_invrt:
   forall p i tt,
-        strip p (L2.term.TInd i) = Ret tt -> tt = (TInd i).
+        strip p (L2.compile.TInd i) = Ret tt -> tt = (TInd i).
 Proof.
   induction tt;  simpl; intros; try discriminate.
   myInjection H. reflexivity.
