theories/L2_typeStripped/awndEval.v
@@ -1,0 +1,220 @@
+(** An alternative definition of wndEval that is extensionally
+*** equivalent for well-formed programs
+**)
+
+(****)
+Add LoadPath "../common" as Common.
+Add LoadPath "../L1_5_box" as L1_5.
+Add LoadPath "../L2_typeStripped" as L2.
+(****)
+
+Require Import Coq.Lists.List.
+Require Import Coq.Strings.String.
+Require Import Coq.Strings.Ascii.
+Require Import Coq.Arith.Compare_dec.
+Require Import Coq.Relations.Relation_Operators.
+Require Import Coq.Relations.Operators_Properties.
+Require Import Coq.Setoids.Setoid.
+Require Import L2.term.
+Require Import L2.program.
+
+Local Open Scope string_scope.
+Local Open Scope bool.
+Local Open Scope list.
+Set Implicit Arguments.
+
+(*** alrernative non-deterministic small step evaluation relation ***)
+Section Env.
+Variable p:environ.
+Inductive awndEval : Term -> Term -> Prop :=
+(** contraction steps **)
+| aConst: forall (s:string) (t:Term),
+         WFapp t -> LookupDfn s p t -> awndEval (TConst s) t
+| aBeta: forall (nm:name) (bod arg:Term) (args:Terms),
+           awndEval (TApp (TLambda nm bod) arg args)
+                   (whBetaStep bod arg args)
+     (* note: [instantiate] is total *)
+| aLetIn: forall (nm:name) (dfn bod:Term),
+            awndEval (TLetIn nm dfn bod) (instantiate dfn 0 bod)
+     (* Case argument must be in Canonical form *)
+     (* np is the number of parameters of the datatype *)
+| aCase: forall (ml:nat * list nat) (s mch:Term)
+                 (args brs ts:Terms) (n:nat),
+            canonicalP mch = Some (n, args) ->
+            tskipn (fst ml) args = Some ts ->
+            whCaseStep n ts brs = Some s ->
+            awndEval (TCase ml mch brs) s
+| aFix: forall (dts:Defs) (m:nat) (arg:Term) (args:Terms)
+               (x:Term) (ix:nat),
+          (** ix is index of recursive argument **)
+          dnthBody m dts = Some (x, ix) ->
+          awndEval (TApp (TFix dts m) arg args)
+                   (pre_whFixStep x dts (tcons arg args))
+| aCast: forall t, awndEval (TCast t) t
+(** congruence steps **)
+(** no xi rules: sLambdaR, sProdR, sLetInR,
+*** no congruence on Case branches or Fix ***)
+| aAppFn:  forall (t r arg:Term) (args:Terms),
+              awndEval t r ->
+              awndEval (mkApp t (tcons arg args)) (mkApp r (tcons arg args))
+| aAppArgs: forall (t arg brg:Term) (args brgs:Terms),
+              awndEvals (tcons arg args) (tcons brg brgs) ->
+              awndEval (TApp t arg args) (TApp t brg brgs)
+| aLetInDef:forall (nm:name) (d1 d2 bod:Term),
+              awndEval d1 d2 ->
+              awndEval (TLetIn nm d1 bod) (TLetIn nm d2 bod)
+| aCaseArg: forall (ml:nat * list nat) (mch can:Term) (brs:Terms),
+              awndEval mch can ->
+              awndEval (TCase ml mch brs) (TCase ml can brs)
+| aCaseBrs: forall (ml:nat * list nat) (mch:Term) (brs brs':Terms),
+              awndEvals brs brs' ->
+              awndEval (TCase ml mch brs) (TCase ml mch brs')
+| aFixDefs: forall (ds es:Defs) (i:nat),
+              awndDEvals ds es -> awndEval (TFix ds i) (TFix es i)
+with awndEvals : Terms -> Terms -> Prop :=
+     | aaHd: forall (t r:Term) (ts:Terms), 
+               awndEval t r ->
+               awndEvals (tcons t ts) (tcons r ts)
+     | aaTl: forall (t:Term) (ts ss:Terms),
+               awndEvals ts ss ->
+               awndEvals (tcons t ts) (tcons t ss)
+with awndDEvals : Defs -> Defs -> Prop :=
+     | adaHd: forall (n:name) (t r:Term) (i:nat) (ds:Defs), 
+               awndEval t r ->
+               awndDEvals (dcons n t i ds) (dcons n r i ds)
+     | adaTl: forall (n:name) (t:Term) (i:nat) (ds es:Defs),
+               awndDEvals ds es ->
+               awndDEvals (dcons n t i ds) (dcons n t i es).
+Hint Constructors awndEval awndEvals awndDEvals.
+Scheme awndEval1_ind := Induction for awndEval Sort Prop
+     with awndEvals1_ind := Induction for awndEvals Sort Prop
+     with awndDEvals1_ind := Induction for awndDEvals Sort Prop.
+Combined Scheme awndEvalEvals_ind
+         from awndEval1_ind, awndEvals1_ind, awndDEvals1_ind.
+
+Definition no_awnd_step (t:Term) : Prop :=
+  no_step awndEval t.
+Definition no_awnds_step (ts:Terms) : Prop :=
+  no_step awndEvals ts.
+
+Lemma awndEval_tappendl:
+  forall bs cs, awndEvals bs cs ->
+  forall ds, awndEvals (tappend bs ds) (tappend cs ds).
+Proof.
+  induction 1; intros.
+  - constructor. assumption.
+  - simpl. apply aaTl. apply IHawndEvals.
+Qed.
+
+Lemma awndEval_tappendr:
+  forall bs cs, awndEvals bs cs ->
+  forall ds, awndEvals (tappend ds bs) (tappend ds cs).
+Proof.
+  intros bs cs h ds. induction ds; simpl.
+  - assumption.
+  - apply aaTl. apply IHds.
+Qed.
+
+Lemma awndEval_Lam_inv:
+  forall nm bod s,
+    awndEval (TLambda nm bod) s -> s = (TLambda nm bod).
+intros nm bod s h. inversion_Clear h. 
+- assert (j:= mkApp_isApp t arg args).
+  destruct j as [x0 [x1 [x2 k]]]. rewrite k in H. discriminate.
+Qed.
+
+Lemma awndEval_Prod_inv:
+  forall nm bod s,
+    awndEval (TProd nm bod) s -> s = (TProd nm bod).
+intros nm bod s h. inversion_Clear h.
+- assert (j:= mkApp_isApp t arg args).
+  destruct j as [x0 [x1 [x2 k]]]. rewrite k in H. discriminate.
+Qed.
+
+Lemma awndEval_Cast_inv:
+  forall tm s, awndEval (TCast tm) s -> tm = s.
+  inversion 1.
+  - reflexivity.
+  - destruct (mkApp_isApp t arg args) as [x0 [x1 [x2 j]]].
+    rewrite H0 in j. discriminate.
+Qed.
+
+Lemma awndEval_pres_WFapp:
+  (forall t s, awndEval t s -> WFapp t -> WFapp s) /\
+  (forall ts ss, awndEvals ts ss -> WFapps ts -> WFapps ss) /\
+  (forall ds es, awndDEvals ds es -> WFappDs ds -> WFappDs es) .
+Proof.
+  apply awndEvalEvals_ind; intros; try assumption;
+  try (solve [inversion_Clear H0; constructor; intuition]).
+  - inversion_Clear H. inversion_Clear H4.
+    apply whBetaStep_pres_WFapp; assumption.
+  - inversion_Clear H. apply instantiate_pres_WFapp; assumption.
+  - inversion_Clear H.
+    refine (whCaseStep_pres_WFapp _ _ _ e1). assumption.
+    refine (tskipn_pres_WFapp _ _ e0).
+    refine (canonicalP_pres_WFapp _ e). assumption.
+  - inversion_Clear H. inversion_Clear H4.
+    assert (j:= dnthBody_pres_WFapp H0 m).
+    apply pre_whFixStep_pres_WFapp; try assumption.
+    + eapply j. eassumption.
+    + constructor; assumption.
+  - inversion_Clear H. assumption.
+  - destruct (WFapp_mkApp_WFapp H0 _ _ eq_refl). inversion_Clear H2.
+    apply mkApp_pres_WFapp.
+    + constructor; assumption.
+    + intuition.
+  - inversion_Clear H0. 
+    assert (j: WFapps (tcons arg args)).
+    { constructor; assumption. }
+    specialize (H j). inversion_Clear H.
+    constructor; assumption.
+Qed.
+
+(** reflexive-transitive closure of wndEval **)
+Inductive awndEvalRTC: Term -> Term -> Prop :=
+(** | wERTCrfl: forall t, WNorm t -> awndEvalRTC p t t ??? **)
+| awERTCrfl: forall t, awndEvalRTC t t
+| awERTCstep: forall t s, awndEval t s -> awndEvalRTC t s
+| awERTCtrn: forall t s u,
+              awndEvalRTC t s -> awndEvalRTC s u -> awndEvalRTC t u.
+Inductive awndEvalsRTC : Terms -> Terms -> Prop :=
+(** | wEsRTCrfl: forall ts, WNorms ts -> wndEvalsRTC p ts ts ??? **)
+| awEsRTCrfl: forall ts, awndEvalsRTC ts ts
+| awEsRTCstep: forall ts ss, awndEvals ts ss -> awndEvalsRTC ts ss
+| awEsRTCtrn: forall ts ss us,
+       awndEvalsRTC ts ss -> awndEvalsRTC ss us -> awndEvalsRTC ts us.
+Inductive awndDEvalsRTC: Defs -> Defs -> Prop :=
+| awDEsRTCrfl: forall ts, awndDEvalsRTC ts ts
+| awDEsRTCstep: forall ts ss, awndDEvals ts ss -> awndDEvalsRTC ts ss
+| awDEsRTCtrn: forall ts ss us, awndDEvalsRTC ts ss -> awndDEvalsRTC ss us ->
+                          awndDEvalsRTC ts us.
+Hint Constructors awndEvalRTC awndEvalsRTC awndDEvalsRTC.
+
+
+Lemma awndEvalRTC_pres_WFapp:
+  forall t s, awndEvalRTC t s -> WFapp t -> WFapp s.
+Proof.
+  induction 1; intros; try assumption.
+  - eapply (proj1 (awndEval_pres_WFapp)); eassumption.
+  - apply IHawndEvalRTC2; try assumption.
+    + apply IHawndEvalRTC1; assumption.
+Qed.
+
+Lemma awndEvalRTC_App_fn:
+  forall fn fn',
+    awndEvalRTC fn fn' -> 
+    forall a1 args,
+      awndEvalRTC (mkApp fn (tcons a1 args)) (mkApp fn' (tcons a1 args)).
+induction 1; intros.
+- apply awERTCrfl.
+- constructor. apply aAppFn. assumption.
+- eapply awERTCtrn. 
+  + apply IHawndEvalRTC1.
+  + apply IHawndEvalRTC2.
+Qed.
+
+
+End Env.
+Hint Constructors awndEval awndDEvals awndEvals.
+Hint Constructors awndEvalRTC awndEvalsRTC awndDEvalsRTC.
+
