theories/L2_typeStripped/compile.v
@@ -1,0 +1,129 @@
+(****)
+Add LoadPath "../common" as Common.
+Add LoadPath "../L1_5_box" as L1_5.
+(****)
+
+Require Import Coq.Lists.List.
+Require Import Coq.Strings.String.
+Require Import Coq.Arith.Compare_dec.
+Require Import Coq.Arith.Peano_dec.
+Require Import Common.Common.
+Require Import L1_5.compile.
+
+Local Open Scope string_scope.
+Local Open Scope bool.
+Local Open Scope list.
+Set Implicit Arguments.
+
+Definition L1_5Term := L1_5.compile.Term.
+Definition L1_5Terms := L1_5.compile.Terms.
+Definition L1_5Defs := L1_5.compile.Defs.
+Definition L1_5EC := L1_5.compile.envClass.
+Definition L1_5Env := L1_5.compile.environ.
+Definition L1_5Pgm := L1_5.compile.Program.
+
+
+Inductive Term : Type :=
+| TRel       : nat -> Term
+| TSort      : Srt -> Term
+| TProof     : Term
+| TCast      : Term -> Term
+| TProd      : name -> Term -> Term
+| TLambda    : name -> Term -> Term
+| TLetIn     : name -> Term -> Term -> Term
+| TApp       : Term -> Term (* first arg must exist *) -> Terms -> Term
+| TConst     : string -> Term
+| TInd       : inductive -> Term
+| TConstruct : inductive -> nat (* cnstr no *) -> Term
+| TCase      : (nat * list nat) (* # parameters, # args per branch *) ->
+               Term -> Terms -> Term
+| TFix       : Defs -> nat -> Term
+with Terms : Type :=
+| tnil : Terms
+| tcons : Term -> Terms -> Terms
+with Defs : Type :=
+| dnil : Defs
+| dcons : name -> Term -> nat -> Defs -> Defs.
+Hint Constructors Term Terms Defs.
+Scheme Trm_ind' := Induction for Term Sort Prop
+  with Trms_ind' := Induction for Terms Sort Prop
+  with Defs_ind' := Induction for Defs Sort Prop.
+Scheme Trm_ind2 := Induction for Term Sort Type
+  with Trms_ind2 := Induction for Terms Sort Type
+  with Defs_ind2 := Induction for Defs Sort Type.
+Combined Scheme TrmTrmsDefs_ind from Trm_ind', Trms_ind', Defs_ind'.
+Combined Scheme TrmTrms_ind from Trm_ind', Trms_ind'.
+Definition tunit (t:Term) : Terms := (tcons t tnil).
+Notation prop := (TSort SProp).
+Notation set_ := (TSort SSet).
+Notation type_ := (TSort SType).
+Notation x_ := (nAnon).
+
+
+Function strip (t:L1_5Term) : Term :=
+  match t with
+    | L1_5.compile.TProof => TProof
+    | L1_5.compile.TRel n => TRel n
+    | L1_5.compile.TSort s => TSort s
+    | L1_5.compile.TCast t _ _ => TCast (strip t)
+    | L1_5.compile.TProd nm _ bod => TProd nm (strip bod)
+    | L1_5.compile.TLambda nm _ bod => TLambda nm (strip bod)
+    | L1_5.compile.TLetIn nm dfn _ bod =>
+      TLetIn nm (strip dfn) (strip bod)
+    | L1_5.compile.TApp fn arg args =>
+      TApp (strip fn) (strip arg) (strips args)
+    | L1_5.compile.TConst nm => TConst nm
+    | L1_5.compile.TInd i => TInd i
+    | L1_5.compile.TConstruct i m => TConstruct i m
+    | L1_5.compile.TCase n _ mch brs => TCase n (strip mch) (strips brs)
+    | L1_5.compile.TFix ds n => TFix (stripDs ds) n
+  end
+with strips (ts:L1_5Terms) : Terms := 
+  match ts with
+    | L1_5.compile.tnil => tnil
+    | L1_5.compile.tcons t ts => tcons (strip t) (strips ts)
+  end
+with stripDs (ts:L1_5Defs) : Defs := 
+  match ts with
+    | L1_5.compile.dnil => dnil
+    | L1_5.compile.dcons nm _ t m ds => dcons nm (strip t) m (stripDs ds)
+  end.
+
+
+(** this function for use in translation from L2 to L3 **)
+Fixpoint arity_from_dtyp
+        (npars:nat) (itps:itypPack) (tndx:nat) (cndx:nat) : exception nat :=
+  do ity <- exnNth itps tndx;
+  do itp <- exnNth (itypCnstrs ity) cndx;
+  ret (npars + (CnstrArity itp)).
+
+(** environments and programs **)
+Definition envClass := AstCommon.envClass Term.
+Definition environ := AstCommon.environ Term.
+Definition Program := AstCommon.Program Term.
+
+Function stripEC (ec:L1_5EC) : envClass :=
+  match ec with
+    | ecTrm _ t => ecTrm Term (strip t)
+    | ecTyp _ n itp => ecTyp Term n itp
+    | ecAx _ => ecAx Term
+  end.
+
+Definition  stripEnv : L1_5Env -> environ :=
+  List.map (fun nmec : string * L1_5EC => (fst nmec, stripEC (snd nmec))).
+
+Definition stripProgram (p:L1_5Pgm) : Program :=
+  {| env:= stripEnv (env _ p);
+     main:= strip (main _ p) |}.
+
+(*** from L0 to L2 ***)
+Definition program_Program (pgm:program) : option Program :=
+  match L1_5.compile.program_Program pgm with
+    | Exc str => None
+    | Ret pgm => Some (stripProgram pgm)
+  end.
+Definition term_Term (t:term) : option Term :=
+  match L1_5.compile.term_Term t with
+    | Exc str => None
+    | Ret trm => Some (strip trm)
+  end.
