theories/L3_flattenedApp/compile.v
@@ -1,0 +1,287 @@
+(******)
+Add LoadPath "../common" as Common.
+Add LoadPath "../L1_5_box" as L1_5.
+Add LoadPath "../L2_typeStripped" as L2.
+(******)
+
+Require Import Coq.Lists.List.
+Require Import Coq.Strings.String.
+Require Import Coq.Arith.Compare_dec.
+Require Import Coq.Arith.Peano_dec.
+Require Import Common.Common.
+Require Import L2.compile.
+Require L2.program.
+
+Local Open Scope string_scope.
+Local Open Scope bool.
+Local Open Scope list.
+Set Implicit Arguments.
+
+Definition L2Term := L2.compile.Term.
+Definition L2Terms := L2.compile.Terms.
+Definition L2Defs := L2.compile.Defs.
+Definition L2EC := L2.compile.envClass.
+Definition L2Env := L2.compile.environ.
+Definition L2Pgm := L2.compile.Program.
+
+
+Inductive Term : Type :=
+| TRel       : nat -> Term
+| TSort      : Srt -> Term
+| TProof     : Term
+| TProd      : name -> Term -> Term
+| TLambda    : name -> Term -> Term
+| TLetIn     : name -> Term -> Term -> Term
+| TApp       : Term -> Term -> Term
+| TConst     : string -> Term
+| TAx        : Term
+| TInd       : inductive -> Term
+| TConstruct : inductive -> nat -> Terms -> Term
+| TCase      : nat * list nat (* #parameters, args per branch *) ->
+               Term -> Terms -> Term
+| TFix       : Defs -> nat -> Term
+with Terms : Type :=
+| tnil : Terms
+| tcons : Term -> Terms -> Terms
+with Defs : Type :=
+| dnil : Defs
+| dcons : name -> Term -> nat -> Defs -> Defs.
+Hint Constructors Term Terms Defs.
+Scheme Trm_ind' := Induction for Term Sort Prop
+  with Trms_ind' := Induction for Terms Sort Prop
+  with Defs_ind' := Induction for Defs Sort Prop.
+Combined Scheme TrmTrmsDefs_ind from Trm_ind', Trms_ind', Defs_ind'.
+Combined Scheme TrmTrms_ind from Trm_ind', Trms_ind'.
+Notation prop := (TSort SProp).
+Notation set_ := (TSort SSet).
+Notation type_ := (TSort SType).
+Notation tunit t := (tcons t tnil).
+
+Fixpoint tlength (ts:Terms) : nat :=
+  match ts with 
+    | tnil => 0
+    | tcons _ ts => S (tlength ts)
+  end.
+
+Fixpoint tappend (ts1 ts2:Terms) : Terms :=
+  match ts1 with
+    | tnil => ts2
+    | tcons t ts => tcons t (tappend ts ts2)
+  end.
+
+Fixpoint dlength (ts:Defs) : nat :=
+  match ts with 
+    | dnil => 0
+    | dcons _ _ _ ts => S (dlength ts)
+  end.
+
+
+(** turn (App fn [x1;...;xn]) into (App (... (App fn x1) x2 ...) xn) **)
+Function mkApp (fn:Term) (xs:Terms) : Term :=
+    match xs with
+      | tnil => fn
+      | tcons b ys => mkApp (TApp fn b) ys
+    end.
+
+(** turn (Constructor [x1;...;xn; 0;...k]])  with arity n+k into
+*** (Lam ... (Lam (Const [x1;...;xn; 0;...k])...))
+**)
+Function mkEta (cstr:Term) (xtraArity:nat) : Term :=
+    match xtraArity with
+      | 0 => cstr
+      | S n => mkEta (TLambda nAnon cstr) n
+    end.
+
+Lemma mkEta_under_Lambda:
+  forall n t, mkEta (TLambda nAnon t) n = TLambda nAnon (mkEta t n).
+Proof.
+  induction n; simpl; intros.
+  - reflexivity.
+  - rewrite IHn. reflexivity.
+Qed.
+
+
+(** Lookup constructor arity in L2 environ (to avoid mutual dependency
+*** between converting L2 terms to L3 and L2 environs to L3)
+**)
+Section EtaExpand.
+Variable p:L2.compile.environ.
+
+(** temp: here we assume the type of constructors is evaluated **)
+(** when removing this; also remove L2.program.arity_from_dtyp **)
+Function cnstrArity (i:inductive) (n:nat) : exception nat :=
+  match i with
+    | mkInd str m => L2.program.cnstrArity str m n p
+  end.
+
+(** compute list of variables for eta expanding a constructor
+*** (which may already be partially applied)
+**)
+Function etaArgs (n:nat) : Terms :=
+  match n with
+    | 0 => tnil
+    | S m => tcons (TRel m) (etaArgs m)
+  end.
+
+Function etaExp_cnstr (i:inductive) (n:nat) (args:Terms) : exception Term :=
+  match cnstrArity i n with
+    | Ret arity =>
+      match nat_compare (tlength args) arity with
+        | Eq => Ret (TConstruct i n args)
+        | Lt => let k := arity - (tlength args)
+                in Ret (mkEta (TConstruct i n (tappend args (etaArgs k))) k)
+        | Gt => Exc ("more arguments than constructor arity: "
+                       ++ (nat_to_string (tlength args)) ++ (" ")
+                       ++ (nat_to_string arity))
+      end
+    | Exc x => Exc x
+  end.
+
+Function strip (t:L2Term) : exception Term :=
+  match t with
+    | L2.compile.TProof => Ret TProof
+    | L2.compile.TRel n => Ret (TRel n)
+    | L2.compile.TSort s => Ret (TSort s)
+    | L2.compile.TCast s => strip s
+    | L2.compile.TProd nm bod => 
+      match strip bod with
+        | Ret sbod => Ret (TProd nm sbod)
+        | x => x
+      end
+    | L2.compile.TLambda nm bod =>
+      match strip bod with
+        | Ret sbod => Ret (TLambda nm sbod)
+        | x => x
+      end
+    | L2.compile.TLetIn nm dfn bod => 
+      match strip dfn, strip bod with
+        | Ret sdfn, Ret sbod => Ret (TLetIn nm sdfn sbod)
+        | Exc s, Ret _ => Exc ("strip dfn fails:" ++ s)
+        | Ret _, Exc s => Exc ("strip bod fails:" ++ s)
+        | Exc s1, Exc s2 => Exc "both strip dfn and strip bod fail"
+      end
+    | L2.compile.TApp fn arg args =>
+      match strip arg, strips args with
+        | Ret sarg, Ret sargs =>
+          match fn with 
+            | L2.compile.TConstruct i n => etaExp_cnstr i n (tcons sarg sargs)
+            | x => match strip x with
+                     | Ret sx => Ret (mkApp sx (tcons sarg sargs))
+                     | x => x
+                   end
+          end
+        | Exc s, Ret _ => Exc ("strip arg fails:" ++ s)
+        | Ret _, Exc s => Exc ("strips args fails:" ++ s)
+        | Exc s1, Exc s2 => Exc "both strip arg and strips args fail"
+      end
+    | L2.compile.TConst nm =>
+      match L2.program.lookup nm p with
+        | Some (AstCommon.ecTrm _ _) => Ret (TConst nm)
+        | Some (AstCommon.ecAx _) => Ret (TAx)
+        | Some (AstCommon.ecTyp _ _ _) =>
+          Exc "L2.compile.lookup nm p returns a type"
+        | None => Exc "L2.compile.lookup nm p misses"
+      end
+    | L2.compile.TInd i => Ret (TInd i)
+    | L2.compile.TConstruct i n => etaExp_cnstr i n tnil
+    | L2.compile.TCase n mch brs =>
+      match strip mch, strips brs with
+        | Ret smch, Ret sbrs => Ret (TCase n smch sbrs)
+        | Exc s, Ret _ => Exc ("strip mch fails:" ++ s)
+        | Ret _, Exc s => Exc ("strips brs fails:" ++ s)
+        | Exc s1, Exc s2 => Exc "both strip mch and strips brs fail"
+      end
+    | L2.compile.TFix ds n =>
+      match stripDs ds with
+        | Ret sds => Ret (TFix sds n)
+        | Exc s => Exc "stripDs ds fails"
+      end
+   end
+with strips (ts:L2Terms) : exception Terms := 
+  match ts with
+    | L2.compile.tnil => Ret tnil
+    | L2.compile.tcons t ts =>
+      match strip t, strips ts with
+        | Ret st, Ret sts => Ret (tcons st sts)
+        | Exc s, Ret _ => Exc ("strip t fails:" ++ s)
+        | Ret _, Exc s => Exc ("strips ts fails:" ++ s)
+        | Exc s1, Exc s2 => Exc "both strip t and strips ts fail"
+      end
+  end
+with stripDs (ts:L2Defs) : exception Defs := 
+  match ts with
+    | L2.compile.dnil => Ret dnil
+    | L2.compile.dcons nm t m ds =>
+      match strip t, stripDs ds with
+        | Ret st, Ret sds => Ret (dcons nm st m sds)
+        | Exc s, Ret _ => Exc ("strip t fails:" ++ s)
+        | Ret _, Exc s => Exc ("stripDs ds fails:" ++ s)
+        | Exc s1, Exc s2 => Exc "both strip t and stripDs ds fail"
+      end
+  end.
+(**
+Functional Scheme strip_ind' := Induction for strip Sort Prop
+with strips_ind' := Induction for strips Sort Prop
+with stripDs_ind' := Induction for stripDs Sort Prop.
+Combined Scheme stripStripsStripDs_ind
+         from strip_ind', strips_ind', stripDs_ind'.
+***)
+
+
+(** environments and programs: no axioms in L3 environments **)
+Inductive envClass := 
+| ecTrm (_:Term)
+| ecTyp (_:nat) (_:itypPack).
+
+(** An environ is a list of definitions.
+***  Currently ignoring Types and Axioms **)
+Definition environ := list (string * envClass).
+Record Program : Type := mkPgm { main:Term; env:environ }.
+
+
+Function stripEC (ec:L2EC) : exception envClass :=
+  match ec with
+    | AstCommon.ecTrm _ t =>
+      match strip t with
+        | Ret u => ret (ecTrm u)
+        | Exc s => raise ("L3.compile, stripEC: " ++ s)
+      end
+    | AstCommon.ecTyp _ n itp => ret (ecTyp n itp)
+    | AstCommon.ecAx _ => raise "stripEC, Anomaly"
+  end.
+
+End EtaExpand.
+
+Function stripEnv (p:L2Env) : exception environ :=
+  match p with
+    | nil => Ret nil
+    | cons (nm, AstCommon.ecAx _) q =>   (** remove axioms from env **)
+      stripEnv q
+    | cons (nm, ec) q =>
+      match stripEC q ec, stripEnv q with
+        | Ret u, Ret r => Ret (cons (nm, u) r)
+        | Exc s, Ret _ => Exc ("strip q t fails:" ++ s)
+        | Ret _, Exc s => Exc ("stripEnv q fails:" ++ s)
+        | Exc s1, Exc s2 => Exc "both strip q t and stripEnv q fail"
+      end
+  end.
+
+Definition stripProgram (p:L2Pgm) : exception Program :=
+  match stripEnv (AstCommon.env _ p),
+        strip (AstCommon.env _ p) (AstCommon.main _ p) with
+    | Ret q, Ret t => ret {| env:= q; main:= t |}
+    | _, _ => raise ("L3 stripProgram; fails")
+  end.
+
+
+(** L0-to-L3 translations **)
+Definition program_Program (p:program) : exception Program :=
+  match L2.compile.program_Program p with
+    | Some q => stripProgram q
+    | None => raise ("L3 program_Program")
+  end.
+Definition term_Term (e:L2.compile.environ) (t:term) : exception Term :=
+  match L2.compile.term_Term t with
+    | None => raise "L2.compile.term_Term failed"
+    | Some trm => strip e trm
+  end.
