theories/L3_flattenedApp/wNorm.v
@@ -2,7 +2,8 @@
 (******)
 Add LoadPath "../common" as Common.
 Add LoadPath "../L1_MalechaQuoted" as L1.
-Add LoadPath "../L2_typeStrippedL1" as L2.
+Add LoadPath "../L1_5_box" as L1_5.
+Add LoadPath "../L2_typeStripped" as L2.
 Add LoadPath "../L3_flattenedApp" as L3.
 (******)
 
@@ -15,6 +16,7 @@ Require Import L3.term.
 Require Import L3.program.
 Require Import L3.wndEval.
 Require Import L3.wcbvEval.
+Require Import L3.compile.
 
 Local Open Scope string_scope.
 Local Open Scope bool.
@@ -28,7 +30,7 @@ Inductive WNorm: Term -> Prop :=
 | WNLam: forall nm bod, WNorm (TLambda nm bod)
 | WNProd: forall nm bod, WNorm (TProd nm bod)
 | WNFix: forall ds br, WNorm (TFix ds br)
-| WNAx: forall nm, WNorm (TAx nm)
+| WNAx: WNorm TAx
 | WNCase: forall mch n brs,
             WNorm mch -> WNorms brs -> ~ isConstruct mch ->
             WNorm (TCase n mch brs)
