theories/L6_PCPS/tests.v
@@ -16,7 +16,7 @@ Require Import ExtLib.Structures.Monads ExtLib.Data.Monads.StateMonad.
 
 Add LoadPath "../common" as Common.
 Add LoadPath "../L1_MalechaQuoted" as L1.
-Add LoadPath "../L2_typeStrippedL1" as L2.
+Add LoadPath "../L2_typeStripped" as L2.
 Add LoadPath "../L3_flattenedApp" as L3.
 Add LoadPath "../L4_deBruijn" as L4.
 Add LoadPath "../L5_CPS" as CPS.
